theories/Template/TermUtils.v
@@ -1,0 +1,42 @@
+From MetaCoq.Lob Require Import Util.Lists.Definitions.
+From MetaCoq.Template Require Import Ast utils.
+
+(** [closenl [x₁;...;xₙ] k c] abstracts over variables [x₁;...;xₙ] and replaces them with
+    [Rel(k); ...; Rel(k+n-1)] in [c]. If two names are identical, the one of least index is kept. *)
+Definition closenl (ids : list ident) : forall (k : nat) (t : term), term
+  := fix closenl (k : nat) (t : term) : term
+    := match t with
+       | tRel _
+       | tSort _
+       | tConstruct _ _ _
+       | tInt _
+       | tFloat _
+       | tConst _ _
+       | tInd _ _
+         => t
+       | tVar id
+         => match List.find_index (String.eqb id) ids with
+            | Some n => tRel (n + k)
+            | None => t
+            end
+       | tEvar ev args => tEvar ev (List.map (closenl k) args)
+       | tLambda na T M => tLambda na (closenl k T) (closenl (S k) M)
+       | tApp u v => mkApps (closenl k u) (List.map (closenl k) v)
+       | tProd na A B => tProd na (closenl k A) (closenl (S k) B)
+       | tCast c kind ty => tCast (closenl k c) kind (closenl k ty)
+       | tLetIn na b ty b' => tLetIn na (closenl k b) (closenl k ty) (closenl (S k) b')
+       | tProj p c => tProj p (closenl k c)
+       | tFix mfix idx =>
+           let k' := List.length mfix + k in
+           let mfix' := List.map (map_def (closenl k) (closenl k')) mfix in
+           tFix mfix' idx
+       | tCoFix mfix idx =>
+           let k' := List.length mfix + k in
+           let mfix' := List.map (map_def (closenl k) (closenl k')) mfix in
+           tCoFix mfix' idx
+       | tCase ind p c brs =>
+           let k' := List.length (pcontext p) + k in
+           let p' := map_predicate id (closenl k) (closenl k') p in
+           let brs' := map_branches_k (closenl) k brs in
+           tCase ind p' (closenl k c) brs'
+       end.
