theories/Util/Lists/Definitions.v
@@ -1,0 +1,9 @@
+Require Import Coq.Lists.List.
+
+Module List.
+  Definition enumerate {A} (ls : list A) : list (nat * A)
+    := combine (seq 0 (length ls)) ls.
+
+  Definition find_index {A} (f : A -> bool) (xs : list A) : option nat
+    := option_map (@fst _ _) (find (fun v => f (snd v)) (enumerate xs)).
+End List.
